reorganizing files

8_extract/main.ml
@@ -10,7 +10,7 @@ open ITreeDefinition
 open Any
 open ImpPrelude
 open ModSem
-open ModSemE
+open Events
 
 (* open MutFG
 open Example0
