1_modules/1_definitions/Events.v
@@ -1,0 +1,191 @@
+Require Import Coqlib.
+Require Export sflib.
+Require Export ITreelib.
+Require Export AList.
+Require Import Any.
+Require Export BasicEvents.
+Require Import IRed.
+
+From Ordinal Require Export Ordinal Arithmetic Inaccessible.
+
+Set Implicit Arguments.
+
+Section ORD.
+  Inductive ord: Type :=
+  | ord_pure (n: Ord.t)
+  | ord_top
+  .
+
+  Definition is_pure (o: ord): bool := match o with | ord_pure _ => true | _ => false end.
+  
+  Definition ord_lt (next cur: ord): Prop :=
+    match next, cur with
+    | ord_pure next, ord_pure cur => (next < cur)%ord
+    | _, ord_top => True
+    | _, _ => False
+    end.
+
+  Definition ord_eval (tbr: bool) (o: ord): Prop :=
+    match tbr with
+    | true => is_pure o
+    | false => o = ord_top
+    end.
+
+End ORD.
+
+Section FSPEC.
+  Context `{Σ: GRA.t}.
+
+  Record fspec: Type := mk_fspec {
+    meta: Type;
+    measure: meta -> ord;
+    precond: meta -> Any.t -> Any_tgt -> iProp; (*** meta-variable -> new logical arg -> current logical arg -> resource arg -> Prop ***)
+    postcond: meta -> Any.t -> Any_tgt -> iProp; (*** meta-variable -> new logical ret -> current logical ret -> resource ret -> Prop ***)
+  }.
+
+  Definition mk (X AA AR: Type) (measure: X -> ord) (precond: X -> AA -> Any_tgt -> iProp) (postcond: X -> AR -> Any_tgt -> iProp) :=
+    @mk_fspec
+      X
+      measure
+      (fun x arg_src arg_tgt => (∃ (aa: AA), ⌜arg_src = aa↑⌝ ∗ precond x aa arg_tgt)%I)
+      (fun x ret_src ret_tgt => (∃ (ar: AR), ⌜ret_src = ar↑⌝ ∗ postcond x ar ret_tgt)%I).
+
+
+  Definition fspec_trivial: fspec :=
+    mk_fspec (meta:=unit) (fun _ => ord_top) (fun _ argh argl => (⌜argh = argl⌝: iProp)%I)
+             (fun _ reth retl => (⌜reth = retl⌝: iProp)%I).
+             
+End FSPEC.
+
+Section HOARE.
+  Context `{Σ: GRA.t}.
+
+  Variant hAPCE: Type -> Type :=
+  | hAPC: hAPCE unit.
+
+  Variant hAGE: Type -> Type :=
+  | Assume (P: iProp): hAGE unit
+  | Guarantee (P: iProp): hAGE unit.
+
+  Definition hEs := (hAGE +' hAPCE +' Es).
+  Definition hAGEs := (hAGE +' Es).
+
+  Section APC.
+    Definition HoareCall (tbr: bool) (ord_cur: ord) (fsp: fspec): gname -> Any.t -> (itree hAGEs) Any.t 
+      := 
+      fun fn varg_src =>
+        x <- trigger (Choose fsp.(meta));; 
+  
+        (*** precondition ***)
+        varg_tgt <- trigger (Choose Any_tgt);;
+        let ord_next := fsp.(measure) x in
+        trigger (Guarantee ((fsp.(precond) x varg_src varg_tgt) ∗ ⌜ord_lt ord_next ord_cur⌝%I ∗ (⌜ord_eval tbr ord_next⌝%I)));;;
+
+        (*** call ***)
+        vret_tgt <- trigger (Call fn varg_tgt);; 
+
+        (*** postcondition ***)
+        vret_src <- trigger (Take Any.t);;
+        trigger (Assume (fsp.(postcond) x vret_src vret_tgt));;;
+
+        Ret vret_src.  
+
+    Program Fixpoint _APC (at_most: Ord.t) {wf Ord.lt at_most} : ord -> itree hAGEs unit :=
+      fun ord_cur => 
+        break <- trigger (Choose _);;
+        if break: bool then Ret tt
+        else
+          n <- trigger (Choose Ord.t);;
+          trigger (Choose (n < at_most)%ord);;;
+          '(fn, varg) <- trigger (Choose _);;
+          fsp <- (stb fn)ǃ;;
+          _ <- HoareCall true ord_cur fsp fn varg;;
+          (_APC n) _ ord_cur.
+    Next Obligation. i. auto. Qed.
+    Next Obligation. eapply Ord.lt_well_founded. Qed.
+
+    Definition HoareAPC (ord_cur: ord): itree hAGEs unit :=
+      at_most <- trigger (Choose _);;
+      _APC at_most ord_cur.
+
+    Lemma unfold_APC: forall at_most ord_cur, 
+      _APC at_most ord_cur 
+      = 
+      break <- trigger (Choose _);;
+      if break: bool then Ret tt
+      else
+        n <- trigger (Choose Ord.t);;
+        guarantee (n < at_most)%ord;;;
+        '(fn, varg) <- trigger (Choose _);;
+        fsp <- (stb fn)ǃ;;
+        _ <- HoareCall true ord_cur fsp fn varg;;
+        (_APC n) ord_cur.
+    Proof.
+      i. unfold _APC. rewrite Fix_eq; eauto.
+      { repeat f_equal. extensionality break. destruct break; ss.
+        repeat f_equal. extensionality n.
+        unfold guarantee. rewrite bind_bind.
+        repeat f_equal. extensionality p.
+        rewrite bind_ret_l. repeat f_equal. extensionality x. destruct x. auto. }
+      { i. replace g with f; auto. extensionality o. eapply H. }
+    Qed.
+
+    Global Opaque _APC.
+
+  End APC.
+
+  Section INTERP.
+    Definition handle_hAPCE_hAGEs (ord_cur: ord): hAPCE ~> itree hAGEs :=
+      fun _ '(hAPC) => HoareAPC ord_cur.
+
+    Definition handle_callE_hAGEs ord_cur: callE ~> itree hAGEs :=
+      fun _ '(Call fn arg) => 
+          fsp <- (stb fn)ǃ;;
+          HoareCall false ord_cur fsp fn arg.
+
+    Definition interp_hEs_hAGEs ord_cur: itree hEs ~> itree hAGEs :=
+      interp (case_ (bif:=sum1) (trivial_Handler) (case_ (bif:=sum1) (handle_hAPCE_hAGEs ord_cur)
+                          (case_ (bif:=sum1) (handle_callE_hAGEs ord_cur)
+                                  trivial_Handler))).    
+    Definition HoareFun
+               {X: Type}
+               (D: X -> ord)
+               (P: X -> Any.t -> Any_tgt -> iProp)
+               (Q: X -> Any.t -> Any_tgt -> iProp)
+               (body: Any.t -> itree hEs Any.t): Any_tgt -> itree hAGEs Any_tgt := fun varg_tgt =>
+      x <- trigger (Take X);;
+
+      (* ASSUME *)
+      varg_src <- trigger (Take _);;
+      let ord_cur := D x in
+      trigger (Assume (P x varg_src varg_tgt));;; (*** precondition ***)
+
+      vret_src <- interp_hEs_hAGEs
+                          ord_cur
+                             (match ord_cur with
+                              | ord_pure _ => _ <- trigger hAPC;; trigger (Choose _)
+                              | _ => body (varg_src)
+                              end);;
+
+      (* ASSERT *)
+      vret_tgt <- trigger (Choose Any_tgt);;
+      trigger (Guarantee (Q x vret_src vret_tgt));;; (*** postcondition ***)
+
+      Ret vret_tgt.
+
+    Definition interp_sb_hp (sb: fspecbody): (Any_tgt -> itree hAGEs Any_tgt) :=
+      let fs: fspec := sb.(fsb_fspec) in
+      (HoareFun (fs.(measure)) (fs.(precond)) (fs.(postcond)) (sb.(fsb_body))).
+
+
+
+  End INTERP.
+
+
+
+End HOARE.
+
+Section INTERP.
+
+End INTERP.
+
