1_modules/1_definitions/EventsInterp.v
@@ -1,0 +1,33 @@
+Require Import Coqlib.
+Require Export sflib.
+Require Export ITreelib.
+Require Export AList.
+Require Import Any.
+Require Import Events.
+
+Set Implicit Arguments.
+
+Section EVENTS.
+  Section INTERP.
+    Definition pure_state {S E}: E ~> stateT S (itree E) := fun _ e s => x <- trigger e;; Ret (s, x).
+    
+    Definition handle_sE {E}: sE ~> stateT Any.t (itree E) := 
+      fun _ e glob =>
+        match e with
+        | SUpdate run => Ret (run glob)
+        end.
+    Definition interp_sE {E}: itree (sE +' E) ~> stateT Any.t (itree E) := 
+      State.interp_state (case_ handle_sE pure_state).
+
+    Definition interp_Es A (prog: callE ~> itree Es) (itr0: itree Es A) (st0: Any.t): itree eventE (Any.t * _)%type :=
+      '(st1, v) <- interp_sE (interp_mrec prog itr0) st0;; Ret (st1, v).
+
+    (* LEMMAS *)
+    Lemma unfold_interp_state: forall {E F} {S R} (h: E ~> stateT S (itree F)) (t: itree E R) (s: S),
+      interp_state h t s = _interp_state h (observe t) s.
+    Proof. i. f. apply unfold_interp_state. Qed.
+
+
+  End INTERP.
+
+End EVENTS.
